## C-4.22

First, we can turn this summation into definite integral.

$$
\sum_{i = 1}^{n}{\lceil \log_{2}{i} \rceil} = \int_{1}^{n}{\lceil \log_{2}{i} \rceil dx} \text{, for } n \in \mathbb N.
$$

Also, we have

$$
\int_{1}^{n}{(\log_{2}{i}) di} < \int_{1}^{n}{\lceil \log_{2}{i} \rceil di} < \int_{1}^{n}{(\log_{2}{i} + 1) di}
$$

By the $\log$ operation

$$
\int_{1}^{n}{(\log_{2}{i}) di} = \frac{1}{\ln(2)}\int_{1}^{n}{\ln{(i)} di}.
$$

Using integration by part, we have

$$
\int_{1}^{n}{\ln{(i)} di} = \left(n \ln n - 0 \right) - \int_{1}^{n}{\left(\frac{1}{i} \times i\right)di} \\ 
= n \ln n - n + 1.
$$

Hence, we found that

$$
n \ln n - n + 1 < \int_{1}^{n}{\lceil \log_{2}{i} \rceil di} < n \ln n + 1.
$$

Since both $n \ln n - n + 1$ and $n \ln n + 1$ are $O(n \log n)$, 

$$
\sum_{i = 1}^{n}{\lceil \log_{2}{i} \rceil} = \int_{1}^{n}{\lceil \log_{2}{i} \rceil dx} \in O(n \log n) \text{, for } n \in \mathbb N.
$$.

### Proof of the intrgration by part

$$
(f(x)g(x))' = f'(x)g(x) + f(x)g'(x)
$$

Using Fundmantal therom of calculus, we have

$$
\int (f(x)g(x))' = \int f'(x)g(x) + \int f(x)g'(x) \\
\Longleftrightarrow f(x)g(x) = \int f'(x)g(x) +  \int f(x)g'(x)\\
\Longleftrightarrow \int f(x)g'(x) = f(x)g(x) - \int f'(x)g(x)
$$

